FreydSSA/Ctx/Var/Fun.lean
@@ -11,9 +11,9 @@ import Mathlib.Order.SuccPred.Basic
 variable {ν ν' α β} [DecidableEq ν] [DecidableEq ν'] [DecidableEq α]
 
 structure FCtx (ν : Type u) (α : Type v) : Type (max u v) where
-  toFun : ν → WithBot α
+  toFun : ν → WithTop α
   support : Finset ν
-  mem_support_toFun : ∀x, x ∈ support ↔ toFun x ≠ ⊥
+  mem_support_toFun : ∀x, x ∈ support ↔ toFun x ≠ ⊤
 
 theorem FCtx.toFun_inj_mp {Γ Δ : FCtx ν α} (h : Γ.toFun = Δ.toFun)
   : Γ = Δ
@@ -31,7 +31,7 @@ theorem FCtx.toFun_inj {Γ Δ : FCtx ν α}
 
 --TODO: Injective instance? Naming convention...
 
-instance FCtx.instFunLike : FunLike (FCtx ν α) ν (WithBot α) where
+instance FCtx.instFunLike : FunLike (FCtx ν α) ν (WithTop α) where
   coe := FCtx.toFun
   coe_injective' := by intro Γ Δ; apply FCtx.toFun_inj_mp
 
@@ -40,7 +40,7 @@ theorem FCtx.ext {Γ Δ : FCtx ν α} (h : ∀x, Γ x = Δ x)
   := DFunLike.coe_injective' (by funext x; apply h)
 
 theorem FCtx.mem_support {Γ : FCtx ν α} (x : ν)
-  : x ∈ Γ.support ↔ Γ x ≠ ⊥ := Γ.mem_support_toFun x
+  : x ∈ Γ.support ↔ Γ x ≠ ⊤ := Γ.mem_support_toFun x
 
 theorem FCtx.isSome_of_mem_support {Γ : FCtx ν α} {x : ν} (h : x ∈ Γ.support) : (Γ x).isSome := by
   simp only [Option.isSome]
@@ -69,19 +69,19 @@ theorem FCtx.mem_support_of_var {Γ : FCtx ν α} (x : ν) (a : α)
   rw [h] at h'
   contradiction
 
-theorem FCtx.not_mem_support_of_eq_bot {Γ : FCtx ν α} (x : ν)
-  (h : Γ x = ⊥) : x ∉ Γ.support := by
+theorem FCtx.not_mem_support_of_eq_top {Γ : FCtx ν α} (x : ν)
+  (h : Γ x = ⊤) : x ∉ Γ.support := by
   rw [mem_support]
   intro h'
   contradiction
 
-theorem FCtx.eq_bot_of_not_mem_support {Γ : FCtx ν α} (x : ν)
-  (h : x ∉ Γ.support) : Γ x = ⊥ := by
+theorem FCtx.eq_top_of_not_mem_support {Γ : FCtx ν α} (x : ν)
+  (h : x ∉ Γ.support) : Γ x = ⊤ := by
   simp [mem_support] at h
   exact h
 
 theorem FCtx.not_mem_support {Γ : FCtx ν α} (x : ν)
-  : x ∉ Γ.support ↔ Γ x = ⊥ := ⟨eq_bot_of_not_mem_support x, not_mem_support_of_eq_bot x⟩
+  : x ∉ Γ.support ↔ Γ x = ⊤ := ⟨eq_top_of_not_mem_support x, not_mem_support_of_eq_top x⟩
 
 def FCtx.map_ty (Γ : FCtx ν α) (f : α → β) : FCtx ν β where
   toFun x := (Γ.toFun x).map (f)
@@ -91,7 +91,7 @@ def FCtx.map_ty (Γ : FCtx ν α) (f : α → β) : FCtx ν β where
     rw [Γ.mem_support_toFun x]
     simp only []
     generalize Γ.toFun x = a
-    cases a <;> simp [WithBot.map, Bot.bot]
+    cases a <;> simp [WithTop.map, Top.top]
 
 def FCtx.cons (x : ν) (a : α) (Γ : FCtx ν α) : FCtx ν α where
   toFun := Function.update Γ.toFun x a
@@ -122,7 +122,7 @@ def FCtx.cons_inj {x : ν} {a a' : α} {Γ : FCtx ν α}
   (h : Γ.cons x a = Γ.cons x a') : a = a' :=
   have hl : Γ.cons x a x = a := by simp [FCtx.cons, DFunLike.coe]
   have hr : Γ.cons x a' x = a' := by simp [FCtx.cons, DFunLike.coe]
-  by rw [<-WithBot.coe_inj, <-hl, <-hr, h]
+  by rw [<-WithTop.coe_inj, <-hl, <-hr, h]
 
 def FCtx.get {Γ : FCtx ν α} {x : ν} (h : x ∈ Γ.support) : α :=
   (Γ x).get (isSome_of_mem_support h)
@@ -151,7 +151,7 @@ theorem FCtx.cons_get_ne (x : ν) (a : α) (Γ : FCtx ν α) (hx : y ≠ x) (hy:
    : (Γ.cons x a).get hy = Γ.get (cons_mem_support_ne x a Γ hx hy)
   := FCtx.get_eq_of hy (cons_mem_support_ne _ _ _ hx hy) (by simp [cons_app, hx])
 
-def FCtx.Wk (Γ Δ : FCtx ν α) : Prop := ∀x, Δ x = ⊥ ∨ Δ x = Γ x
+def FCtx.Wk (Γ Δ : FCtx ν α) : Prop := ∀x, Δ x = ⊤ ∨ Δ x = Γ x
 
 theorem FCtx.Wk.refl (Γ : FCtx ν α) : FCtx.Wk Γ Γ := by simp [FCtx.Wk]
 theorem FCtx.Wk.comp {Γ Δ Θ : FCtx ν α} (w : FCtx.Wk Γ Δ) (w' : FCtx.Wk Δ Θ)
@@ -169,19 +169,19 @@ theorem FCtx.Wk.antisymm {Γ Δ : FCtx ν α} (w : FCtx.Wk Γ Δ) (w' : FCtx.Wk 
 def FCtx.Wk.src {Γ Δ : FCtx ν α} (_ : FCtx.Wk Γ Δ) : FCtx ν α := Γ
 def FCtx.Wk.trg {Γ Δ : FCtx ν α} (_ : FCtx.Wk Γ Δ) : FCtx ν α := Δ
 
-theorem FCtx.Wk.eq_bot {Γ Δ : FCtx ν α} (w : FCtx.Wk Γ Δ) (x : ν) (h : Γ x = ⊥)
-  : Δ x = ⊥ := by cases w x <;> simp [*]
-theorem FCtx.Wk.ne_bot {Γ Δ : FCtx ν α} (w : FCtx.Wk Γ Δ) (x : ν) (h : Δ x ≠ ⊥)
-  : Γ x ≠ ⊥ := λh' => h (w.eq_bot _ h')
-theorem FCtx.Wk.eq_some_ne_bot {Γ Δ : FCtx ν α} (w : FCtx.Wk Γ Δ)
-  (x : ν) (h : Δ x ≠ ⊥)
-  : Γ x ≠ ⊥ := λh' => h (w.eq_bot _ h')
+theorem FCtx.Wk.eq_top {Γ Δ : FCtx ν α} (w : FCtx.Wk Γ Δ) (x : ν) (h : Γ x = ⊤)
+  : Δ x = ⊤ := by cases w x <;> simp [*]
+theorem FCtx.Wk.ne_top {Γ Δ : FCtx ν α} (w : FCtx.Wk Γ Δ) (x : ν) (h : Δ x ≠ ⊤)
+  : Γ x ≠ ⊤ := λh' => h (w.eq_top _ h')
+theorem FCtx.Wk.eq_some_ne_top {Γ Δ : FCtx ν α} (w : FCtx.Wk Γ Δ)
+  (x : ν) (h : Δ x ≠ ⊤)
+  : Γ x ≠ ⊤ := λh' => h (w.eq_top _ h')
 
 theorem FCtx.Wk.support_subset {Γ Δ : FCtx ν α} (w : FCtx.Wk Γ Δ)
   : Δ.support ⊆ Γ.support := by
   intro x
   rw [Γ.mem_support_toFun, Δ.mem_support_toFun]
-  exact w.ne_bot x
+  exact w.ne_top x
 
 -- theorem FCtx.Wk.mem_support {Γ Δ : FCtx ν α} (w : FCtx.Wk Γ Δ)
 --   : ∀{x}, x ∈ Δ.support → x ∈ Γ.support := by
@@ -190,12 +190,14 @@ theorem FCtx.Wk.support_subset {Γ Δ : FCtx ν α} (w : FCtx.Wk Γ Δ)
 --   exact w.ne_bot x
 
 instance FCtx.instPartialOrder : PartialOrder (FCtx ν α) where
-  le a b := FCtx.Wk b a
+  le a b := FCtx.Wk a b
   le_refl := FCtx.Wk.refl
-  le_trans _ _ _ h h' := FCtx.Wk.comp h' h
-  le_antisymm _ _ h h' := FCtx.Wk.antisymm h' h
+  le_trans _ _ _ := FCtx.Wk.comp
+  le_antisymm _ _ := FCtx.Wk.antisymm
 
-def FCtx.Cmp (Δ Δ' : FCtx ν α) : Prop := ∀x, Δ x = Δ' x ∨ Δ x = ⊥ ∨ Δ' x = ⊥
+-- TODO: FCtx.Wk has sup-semilattice structure, via ⊤, but infima do not always exist...
+
+def FCtx.Cmp (Δ Δ' : FCtx ν α) : Prop := ∀x, Δ x = Δ' x ∨ Δ x = ⊤ ∨ Δ' x = ⊤
 
 theorem FCtx.Cmp.refl (Γ : FCtx ν α) : FCtx.Cmp Γ Γ := by simp [FCtx.Cmp]
 
@@ -218,55 +220,55 @@ theorem FCtx.Wk.cmp₂ {Γ Δ Δ' : FCtx ν α} (w : FCtx.Wk Γ Δ) (w' : FCtx.W
   : FCtx.Cmp Δ Δ' := FCtx.Cmp.of_wk₂ w w'
 theorem FCtx.Wk.cmp {Γ Δ : FCtx ν α} (w : FCtx.Wk Γ Δ) : FCtx.Cmp Γ Δ := FCtx.Cmp.of_wk w
 
-def FCtx.linf (Δ Δ' : FCtx ν α)
+def FCtx.lsup (Δ Δ' : FCtx ν α)
   : FCtx ν α where
   toFun x := match Δ x, Δ' x with
-    | ⊥, _ | _, ⊥ => ⊥
+    | ⊤, _ | _, ⊤ => ⊤
     | some a, some _ => some a
   support := Δ.support ∩ Δ'.support
   mem_support_toFun := by
     intro x
     simp only [Finset.mem_inter, mem_support]
-    split <;> simp [Bot.bot, *]
+    split <;> simp [Top.top, *]
 
-theorem FCtx.linf_app (Δ Δ' : FCtx ν α) (x : ν)
-  : (FCtx.linf Δ Δ') x = match Δ x, Δ' x with
-    | ⊥, _ | _, ⊥ => ⊥
+theorem FCtx.lsup_app (Δ Δ' : FCtx ν α) (x : ν)
+  : (FCtx.lsup Δ Δ') x = match Δ x, Δ' x with
+    | ⊤, _ | _, ⊤ => ⊤
     | some a, some _ => some a := by rfl
 
-theorem FCtx.linf_support {Δ Δ' : FCtx ν α}
-  : (FCtx.linf Δ Δ').support = Δ.support ∩ Δ'.support := rfl
-theorem FCtx.linf_mem_support {Δ Δ' : FCtx ν α} (x : ν)
-  : x ∈ (FCtx.linf Δ Δ').support ↔ x ∈ Δ.support ∧ x ∈ Δ'.support := by
-  simp [linf_support]
+theorem FCtx.lsup_support {Δ Δ' : FCtx ν α}
+  : (FCtx.lsup Δ Δ').support = Δ.support ∩ Δ'.support := rfl
+theorem FCtx.lsup_mem_support {Δ Δ' : FCtx ν α} (x : ν)
+  : x ∈ (FCtx.lsup Δ Δ').support ↔ x ∈ Δ.support ∧ x ∈ Δ'.support := by
+  simp [lsup_support]
 
-def FCtx.rinf (Δ Δ' : FCtx ν α)
+def FCtx.rsup (Δ Δ' : FCtx ν α)
   : FCtx ν α where
   toFun x := match Δ x, Δ' x with
-    | ⊥, _ | _, ⊥ => ⊥
+    | ⊤, _ | _, ⊤ => ⊤
     | some _, some a => some a
   support := Δ.support ∩ Δ'.support
   mem_support_toFun := by
     intro x
     simp only [Finset.mem_inter, mem_support]
-    split <;> simp [Bot.bot, *]
+    split <;> simp [Top.top, *]
 
-theorem FCtx.rinf_app (Δ Δ' : FCtx ν α) (x : ν)
-  : (FCtx.rinf Δ Δ') x = match Δ x, Δ' x with
-    | ⊥, _ | _, ⊥ => ⊥
+theorem FCtx.rsup_app (Δ Δ' : FCtx ν α) (x : ν)
+  : (FCtx.rsup Δ Δ') x = match Δ x, Δ' x with
+    | ⊤, _ | _, ⊤ => ⊤
     | some _, some a => some a := by rfl
 
-theorem FCtx.rinf_support {Δ Δ' : FCtx ν α}
-  : (FCtx.rinf Δ Δ').support = Δ.support ∩ Δ'.support := rfl
+theorem FCtx.rsup_support {Δ Δ' : FCtx ν α}
+  : (FCtx.rsup Δ Δ').support = Δ.support ∩ Δ'.support := rfl
 
-theorem FCtx.linf_wk (Δ Δ' : FCtx ν α) : FCtx.Wk Δ (FCtx.linf Δ Δ') := by
+theorem FCtx.lsup_wk (Δ Δ' : FCtx ν α) : FCtx.Wk Δ (FCtx.lsup Δ Δ') := by
   intro x
-  simp [linf_app]
+  simp [lsup_app]
   split <;> simp [*]
 
-theorem FCtx.rinf_wk (Δ Δ' : FCtx ν α) : FCtx.Wk Δ' (FCtx.rinf Δ Δ') := by
+theorem FCtx.rsup_wk (Δ Δ' : FCtx ν α) : FCtx.Wk Δ' (FCtx.rsup Δ Δ') := by
   intro x
-  simp [rinf_app]
+  simp [rsup_app]
   split <;> simp [*]
 
 theorem FCtx.Wk.var_eq {Γ Δ : FCtx ν α} (w : FCtx.Wk Γ Δ) (x : ν) (a b : α)
@@ -295,7 +297,7 @@ theorem FCtx.Cmp.var_eq {Γ Δ : FCtx ν α} (c : FCtx.Cmp Γ Δ) (x : ν) (a b 
 
 theorem FCtx.Wk.var_eq₂' {Γ Δ Δ' : FCtx ν α} (w : FCtx.Wk Γ Δ) (w' : FCtx.Wk Γ Δ')
   (x : ν) (a b : α) (h : Δ x = a) (h' : Δ' x = b)
-  : (a : WithBot α) = (b : WithBot α) := by rw [<-var w x a h, <-var w' x b h']
+  : (a : WithTop α) = (b : WithTop α) := by rw [<-var w x a h, <-var w' x b h']
 
 theorem FCtx.Wk.var_eq₂ {Γ Δ Δ' : FCtx ν α} (w : FCtx.Wk Γ Δ) (w' : FCtx.Wk Γ Δ')
   (x : ν) (a b : α) (h : Δ x = a) (h' : Δ' x = b)
@@ -322,7 +324,7 @@ theorem FCtx.Wk.of_eq_on {Γ Δ : FCtx ν α}
   if h' : x ∈ Δ.support then
     simp [h _ h']
   else
-    simp [eq_bot_of_not_mem_support _ h']
+    simp [eq_top_of_not_mem_support _ h']
 
 theorem FCtx.Wk.eq_on_iff {Γ Δ : FCtx ν α}
   : FCtx.Wk Γ Δ ↔ (∀x ∈ Δ.support, Δ x = Γ x) := ⟨eq_on, of_eq_on⟩
@@ -341,278 +343,278 @@ theorem FCtx.Wk.cons_not_mem (x : ν) (a : α) (Γ : FCtx ν α) (hx : x ∉ Γ.
   simp only [cons_app]
   split <;> simp [<-not_mem_support, *]
 
-theorem FCtx.Cmp.linf_eq_rinf {Δ Δ' : FCtx ν α} (c : FCtx.Cmp Δ Δ')
-  : FCtx.linf Δ Δ' = FCtx.rinf Δ Δ' := by
+theorem FCtx.Cmp.lsup_eq_rsup {Δ Δ' : FCtx ν α} (c : FCtx.Cmp Δ Δ')
+  : FCtx.lsup Δ Δ' = FCtx.rsup Δ Δ' := by
   apply FCtx.ext
   intro x
-  simp only [DFunLike.coe, linf, rinf]
+  simp only [DFunLike.coe, lsup, rsup]
   split
   . rfl
   . rfl
   . apply var_eq' c <;> assumption
 
-theorem FCtx.Wk.linf_eq_rinf {Γ Δ Δ' : FCtx ν α} (w : FCtx.Wk Γ Δ) (w' : FCtx.Wk Γ Δ')
-  : FCtx.linf Δ Δ' = FCtx.rinf Δ Δ' := (w.cmp₂ w').linf_eq_rinf
+theorem FCtx.Wk.lsup_eq_rsup {Γ Δ Δ' : FCtx ν α} (w : FCtx.Wk Γ Δ) (w' : FCtx.Wk Γ Δ')
+  : FCtx.lsup Δ Δ' = FCtx.rsup Δ Δ' := (w.cmp₂ w').lsup_eq_rsup
 
-theorem FCtx.Cmp.linf_wk_left {Δ Δ' : FCtx ν α} (_ : FCtx.Cmp Δ Δ')
-  : FCtx.Wk Δ (FCtx.linf Δ Δ') := linf_wk Δ Δ'
-theorem FCtx.Cmp.linf_wk_right {Δ Δ' : FCtx ν α} (c : FCtx.Cmp Δ Δ')
-  : FCtx.Wk Δ' (FCtx.linf Δ Δ') := c.linf_eq_rinf ▸ rinf_wk Δ Δ'
+theorem FCtx.Cmp.lsup_wk_left {Δ Δ' : FCtx ν α} (_ : FCtx.Cmp Δ Δ')
+  : FCtx.Wk Δ (FCtx.lsup Δ Δ') := lsup_wk Δ Δ'
+theorem FCtx.Cmp.lsup_wk_right {Δ Δ' : FCtx ν α} (c : FCtx.Cmp Δ Δ')
+  : FCtx.Wk Δ' (FCtx.lsup Δ Δ') := c.lsup_eq_rsup ▸ rsup_wk Δ Δ'
 
-theorem FCtx.Wk.linf_wk_left {Γ Δ Δ' : FCtx ν α} (_ : FCtx.Wk Γ Δ) (_ : FCtx.Wk Γ Δ')
-  : FCtx.Wk Δ (FCtx.linf Δ Δ') := linf_wk Δ Δ'
-theorem FCtx.Wk.linf_wk_right {Γ Δ Δ' : FCtx ν α} (w : FCtx.Wk Γ Δ) (w' : FCtx.Wk Γ Δ')
-  : FCtx.Wk Δ' (FCtx.linf Δ Δ') := linf_eq_rinf w w' ▸ rinf_wk Δ Δ'
+theorem FCtx.Wk.lsup_wk_left {Γ Δ Δ' : FCtx ν α} (_ : FCtx.Wk Γ Δ) (_ : FCtx.Wk Γ Δ')
+  : FCtx.Wk Δ (FCtx.lsup Δ Δ') := lsup_wk Δ Δ'
+theorem FCtx.Wk.lsup_wk_right {Γ Δ Δ' : FCtx ν α} (w : FCtx.Wk Γ Δ) (w' : FCtx.Wk Γ Δ')
+  : FCtx.Wk Δ' (FCtx.lsup Δ Δ') := lsup_eq_rsup w w' ▸ rsup_wk Δ Δ'
 
-theorem FCtx.Cmp.rinf_wk_left {Δ Δ' : FCtx ν α} (c : FCtx.Cmp Δ Δ')
-  : FCtx.Wk Δ (FCtx.rinf Δ Δ') := c.linf_eq_rinf ▸ linf_wk Δ Δ'
-theorem FCtx.Cmp.rinf_wk_right {Δ Δ' : FCtx ν α} (_ : FCtx.Cmp Δ Δ')
-  : FCtx.Wk Δ' (FCtx.rinf Δ Δ') := rinf_wk Δ Δ'
+theorem FCtx.Cmp.rsup_wk_left {Δ Δ' : FCtx ν α} (c : FCtx.Cmp Δ Δ')
+  : FCtx.Wk Δ (FCtx.rsup Δ Δ') := c.lsup_eq_rsup ▸ lsup_wk Δ Δ'
+theorem FCtx.Cmp.rsup_wk_right {Δ Δ' : FCtx ν α} (_ : FCtx.Cmp Δ Δ')
+  : FCtx.Wk Δ' (FCtx.rsup Δ Δ') := rsup_wk Δ Δ'
 
-theorem FCtx.Wk.rinf_wk_left {Γ Δ Δ' : FCtx ν α} (w : FCtx.Wk Γ Δ) (w' : FCtx.Wk Γ Δ')
-  : FCtx.Wk Δ (FCtx.rinf Δ Δ') := linf_eq_rinf w w' ▸ linf_wk Δ Δ'
-theorem FCtx.Wk.rinf_wk_right {Γ Δ Δ' : FCtx ν α} (_ : FCtx.Wk Γ Δ) (_ : FCtx.Wk Γ Δ')
-  : FCtx.Wk Δ' (FCtx.rinf Δ Δ') := rinf_wk Δ Δ'
+theorem FCtx.Wk.rsup_wk_left {Γ Δ Δ' : FCtx ν α} (w : FCtx.Wk Γ Δ) (w' : FCtx.Wk Γ Δ')
+  : FCtx.Wk Δ (FCtx.rsup Δ Δ') := lsup_eq_rsup w w' ▸ lsup_wk Δ Δ'
+theorem FCtx.Wk.rsup_wk_right {Γ Δ Δ' : FCtx ν α} (_ : FCtx.Wk Γ Δ) (_ : FCtx.Wk Γ Δ')
+  : FCtx.Wk Δ' (FCtx.rsup Δ Δ') := rsup_wk Δ Δ'
 
-theorem FCtx.linf_eq_none_left {Δ Δ' : FCtx ν α} (x : ν) (h : Δ x = ⊥)
-  : FCtx.linf Δ Δ' x = ⊥ := by
-  simp only [linf_app]
+theorem FCtx.lsup_eq_none_left {Δ Δ' : FCtx ν α} (x : ν) (h : Δ x = ⊤)
+  : FCtx.lsup Δ Δ' x = ⊤ := by
+  simp only [lsup_app]
   split <;> simp only [h] at *
-theorem FCtx.linf_eq_none_right {Δ Δ' : FCtx ν α} (x : ν) (h : Δ' x = ⊥)
-  : FCtx.linf Δ Δ' x = ⊥ := by
-  simp only [linf_app] at *
+theorem FCtx.lsup_eq_none_right {Δ Δ' : FCtx ν α} (x : ν) (h : Δ' x = ⊤)
+  : FCtx.lsup Δ Δ' x = ⊤ := by
+  simp only [lsup_app] at *
   split <;> simp only [h] at *
-theorem FCtx.linf_eq_none_or {Δ Δ' : FCtx ν α} (x : ν) (h : FCtx.linf Δ Δ' x = ⊥)
-  : Δ x = ⊥ ∨ Δ' x = ⊥ := by
-  simp only [linf_app] at h
+theorem FCtx.lsup_eq_none_or {Δ Δ' : FCtx ν α} (x : ν) (h : FCtx.lsup Δ Δ' x = ⊤)
+  : Δ x = ⊤ ∨ Δ' x = ⊤ := by
+  simp only [lsup_app] at h
   rw [<-h] -- hack until term-to-split is supported...
-  split <;> simp [*, Bot.bot]
-theorem FCtx.linf_eq_none_iff {Δ Δ' : FCtx ν α} (x : ν)
-  : FCtx.linf Δ Δ' x = ⊥ ↔ Δ x = ⊥ ∨ Δ' x = ⊥ :=
-  ⟨linf_eq_none_or x, λh => h.elim (linf_eq_none_left x) (linf_eq_none_right x)⟩
+  split <;> simp [*, Top.top]
+theorem FCtx.lsup_eq_none_iff {Δ Δ' : FCtx ν α} (x : ν)
+  : FCtx.lsup Δ Δ' x = ⊤ ↔ Δ x = ⊤ ∨ Δ' x = ⊤ :=
+  ⟨lsup_eq_none_or x, λh => h.elim (lsup_eq_none_left x) (lsup_eq_none_right x)⟩
 
-theorem FCtx.linf_var_left {Δ Δ' : FCtx ν α} (x : ν) (a : α)
-  : FCtx.linf Δ Δ' x = a → Δ x = a := by
-  simp only [linf_app]
+theorem FCtx.lsup_var_left {Δ Δ' : FCtx ν α} (x : ν) (a : α)
+  : FCtx.lsup Δ Δ' x = a → Δ x = a := by
+  simp only [lsup_app]
   split <;> intro h <;> cases h; assumption
-theorem FCtx.linf_var_right {Δ Δ' : FCtx ν α} (x : ν) (a : α)
-  : FCtx.linf Δ Δ' x = a → ∃b : α, Δ' x = b := by
-  simp only [linf_app]
+theorem FCtx.lsup_var_right {Δ Δ' : FCtx ν α} (x : ν) (a : α)
+  : FCtx.lsup Δ Δ' x = a → ∃b : α, Δ' x = b := by
+  simp only [lsup_app]
   split <;> intro h <;> cases h; exact ⟨_, by assumption⟩
 
-theorem FCtx.linf_var_left_eq' {Δ Δ' : FCtx ν α} (x : ν) (a : α) (bb : WithBot α)
-  (h : FCtx.linf Δ Δ' x = a) (h' : Δ x = bb) : a = bb := by
-    rw [<-linf_var_left x a h]; assumption
-theorem FCtx.linf_var_left_eq {Δ Δ' : FCtx ν α} (x : ν) (a b : α)
-  (h : FCtx.linf Δ Δ' x = a) (h' : Δ x = b) : a = b := by
-    cases linf_var_left_eq' x a b h h'; rfl
+theorem FCtx.lsup_var_left_eq' {Δ Δ' : FCtx ν α} (x : ν) (a : α) (bb : WithTop α)
+  (h : FCtx.lsup Δ Δ' x = a) (h' : Δ x = bb) : a = bb := by
+    rw [<-lsup_var_left x a h]; assumption
+theorem FCtx.lsup_var_left_eq {Δ Δ' : FCtx ν α} (x : ν) (a b : α)
+  (h : FCtx.lsup Δ Δ' x = a) (h' : Δ x = b) : a = b := by
+    cases lsup_var_left_eq' x a b h h'; rfl
 
-theorem FCtx.linf_support_eq_left {Δ Δ' : FCtx ν α} (x : ν)
-  (h : x ∈ (linf Δ Δ').support) : FCtx.linf Δ Δ' x = Δ x := (linf_wk Δ Δ').eq_on x h
+theorem FCtx.lsup_support_eq_left {Δ Δ' : FCtx ν α} (x : ν)
+  (h : x ∈ (lsup Δ Δ').support) : FCtx.lsup Δ Δ' x = Δ x := (lsup_wk Δ Δ').eq_on x h
 
-theorem FCtx.linf_var_eq_left {Δ Δ' : FCtx ν α} (x : ν) (a : α)
-  (h : FCtx.linf Δ Δ' x = a)
-  : FCtx.linf Δ Δ' x = Δ x := by
+theorem FCtx.lsup_var_eq_left {Δ Δ' : FCtx ν α} (x : ν) (a : α)
+  (h : FCtx.lsup Δ Δ' x = a)
+  : FCtx.lsup Δ Δ' x = Δ x := by
     rw [h]
     apply Eq.symm
-    apply linf_var_left
+    apply lsup_var_left
     exact h
-theorem FCtx.linf_right_var_eq_left {Δ Δ' : FCtx ν α} (x : ν) (a : α)
+theorem FCtx.lsup_right_var_eq_left {Δ Δ' : FCtx ν α} (x : ν) (a : α)
   (h : Δ' x = a)
-  : FCtx.linf Δ Δ' x = Δ x := by
-    rw [linf_app]
+  : FCtx.lsup Δ Δ' x = Δ x := by
+    rw [lsup_app]
     split
-    . simp [*, Bot.bot] at *
+    . simp [*, Top.top] at *
     . rw [h] at *; contradiction
     . simp [*]
 
-theorem FCtx.linf_some_eq_left {Δ Δ' : FCtx ν α} (x : ν)
-: (∃a : α, FCtx.linf Δ Δ' x = a) → FCtx.linf Δ Δ' x = Δ x := by
+theorem FCtx.lsup_some_eq_left {Δ Δ' : FCtx ν α} (x : ν)
+: (∃a : α, FCtx.lsup Δ Δ' x = a) → FCtx.lsup Δ Δ' x = Δ x := by
   intro ⟨a, h⟩
   rw [h]
   apply Eq.symm
-  apply linf_var_left
+  apply lsup_var_left
   exact h
-theorem FCtx.linf_right_some_eq_left {Δ Δ' : FCtx ν α} (x : ν)
-  : (∃a: α, Δ' x = a) → FCtx.linf Δ Δ' x = Δ x := by
+theorem FCtx.lsup_right_some_eq_left {Δ Δ' : FCtx ν α} (x : ν)
+  : (∃a: α, Δ' x = a) → FCtx.lsup Δ Δ' x = Δ x := by
   intro ⟨a, h⟩
-  apply linf_right_var_eq_left _ _ h
-theorem FCtx.linf_right_support_eq_left {Δ Δ' : FCtx ν α} (x : ν)
-  (h : x ∈ Δ'.support) : FCtx.linf Δ Δ' x = Δ x := by
-  apply linf_right_some_eq_left _ ((mem_support_exists _).mp h)
+  apply lsup_right_var_eq_left _ _ h
+theorem FCtx.lsup_right_support_eq_left {Δ Δ' : FCtx ν α} (x : ν)
+  (h : x ∈ Δ'.support) : FCtx.lsup Δ Δ' x = Δ x := by
+  apply lsup_right_some_eq_left _ ((mem_support_exists _).mp h)
   rfl
-theorem FCtx.linf_left_not_support {Δ Δ' : FCtx ν α} (x : ν)
-  (h : x ∉ Δ.support) : FCtx.linf Δ Δ' x = ⊥ := by
-  apply linf_eq_none_left
-  apply eq_bot_of_not_mem_support
+theorem FCtx.lsup_left_not_support {Δ Δ' : FCtx ν α} (x : ν)
+  (h : x ∉ Δ.support) : FCtx.lsup Δ Δ' x = ⊤ := by
+  apply lsup_eq_none_left
+  apply eq_top_of_not_mem_support
   exact h
-theorem FCtx.linf_right_not_support {Δ Δ' : FCtx ν α} (x : ν)
-  (h : x ∉ Δ'.support) : FCtx.linf Δ Δ' x = ⊥ := by
-  apply linf_eq_none_right
-  apply eq_bot_of_not_mem_support
+theorem FCtx.lsup_right_not_support {Δ Δ' : FCtx ν α} (x : ν)
+  (h : x ∉ Δ'.support) : FCtx.lsup Δ Δ' x = ⊤ := by
+  apply lsup_eq_none_right
+  apply eq_top_of_not_mem_support
   exact h
-theorem FCtx.linf_eq_eq_left {Δ Δ' : FCtx ν α} (x : ν)
-  (h : Δ x = Δ' x) : FCtx.linf Δ Δ' x = Δ x := by
+theorem FCtx.lsup_eq_eq_left {Δ Δ' : FCtx ν α} (x : ν)
+  (h : Δ x = Δ' x) : FCtx.lsup Δ Δ' x = Δ x := by
   if h': x ∈ Δ'.support then
-    rw [linf_right_support_eq_left _ h']
+    rw [lsup_right_support_eq_left _ h']
   else
-    rw [linf_right_not_support _ h']
-    rw [eq_bot_of_not_mem_support _ h'] at h
+    rw [lsup_right_not_support _ h']
+    rw [eq_top_of_not_mem_support _ h'] at h
     rw [h]
-theorem FCtx.linf_eq_eq_right {Δ Δ' : FCtx ν α} (x : ν)
-  (h : Δ x = Δ' x) : FCtx.linf Δ Δ' x = Δ' x := by
-  rw [linf_eq_eq_left _ h]
+theorem FCtx.lsup_eq_eq_right {Δ Δ' : FCtx ν α} (x : ν)
+  (h : Δ x = Δ' x) : FCtx.lsup Δ Δ' x = Δ' x := by
+  rw [lsup_eq_eq_left _ h]
   exact h
 
-theorem FCtx.Wk.linf_wk {Γ Δ Δ' : FCtx ν α} (w : FCtx.Wk Δ Γ) (w' : FCtx.Wk Δ' Γ)
-  : FCtx.Wk (FCtx.linf Δ Δ') Γ := by
+theorem FCtx.Wk.lsup_wk {Γ Δ Δ' : FCtx ν α} (w : FCtx.Wk Δ Γ) (w' : FCtx.Wk Δ' Γ)
+  : FCtx.Wk (FCtx.lsup Δ Δ') Γ := by
   simp only [eq_on_iff] at *
   intro x hx
-  rw [linf_eq_eq_left]
+  rw [lsup_eq_eq_left]
   . rw [<-w _ hx]
   . rw [<-w' _ hx]
     rw [<-w _ hx]
 
-theorem FCtx.rinf_eq_none_left {Δ Δ' : FCtx ν α} (x : ν) (h : Δ x = ⊥)
-  : FCtx.rinf Δ Δ' x = ⊥ := by
-  simp only [rinf_app]
+theorem FCtx.rsup_eq_none_left {Δ Δ' : FCtx ν α} (x : ν) (h : Δ x = ⊤)
+  : FCtx.rsup Δ Δ' x = ⊤ := by
+  simp only [rsup_app]
   split <;> simp only [h] at *
-theorem FCtx.rinf_eq_none_right {Δ Δ' : FCtx ν α} (x : ν) (h : Δ' x = ⊥)
-  : FCtx.rinf Δ Δ' x = ⊥ := by
-  simp only [rinf_app] at *
+theorem FCtx.rsup_eq_none_right {Δ Δ' : FCtx ν α} (x : ν) (h : Δ' x = ⊤)
+  : FCtx.rsup Δ Δ' x = ⊤ := by
+  simp only [rsup_app] at *
   split <;> simp only [h] at *
-theorem FCtx.rinf_eq_none_or {Δ Δ' : FCtx ν α} (x : ν) (h : FCtx.rinf Δ Δ' x = ⊥)
-  : Δ x = ⊥ ∨ Δ' x = ⊥ := by
-  simp only [rinf_app] at h
+theorem FCtx.rsup_eq_none_or {Δ Δ' : FCtx ν α} (x : ν) (h : FCtx.rsup Δ Δ' x = ⊤)
+  : Δ x = ⊤ ∨ Δ' x = ⊤ := by
+  simp only [rsup_app] at h
   rw [<-h] -- hack until term-to-split is supported...
-  split <;> simp [*, Bot.bot]
-theorem FCtx.rinf_eq_none_iff {Δ Δ' : FCtx ν α} (x : ν)
-  : FCtx.rinf Δ Δ' x = ⊥ ↔ Δ x = ⊥ ∨ Δ' x = ⊥ :=
-  ⟨rinf_eq_none_or x, λh => h.elim (rinf_eq_none_left x) (rinf_eq_none_right x)⟩
+  split <;> simp [*, Top.top]
+theorem FCtx.rsup_eq_none_iff {Δ Δ' : FCtx ν α} (x : ν)
+  : FCtx.rsup Δ Δ' x = ⊤ ↔ Δ x = ⊤ ∨ Δ' x = ⊤ :=
+  ⟨rsup_eq_none_or x, λh => h.elim (rsup_eq_none_left x) (rsup_eq_none_right x)⟩
 
-theorem FCtx.rinf_var_left {Δ Δ' : FCtx ν α} (x : ν) (a : α)
-  : FCtx.rinf Δ Δ' x = a → ∃b : α, Δ x = b := by
-  simp only [rinf_app]
+theorem FCtx.rsup_var_left {Δ Δ' : FCtx ν α} (x : ν) (a : α)
+  : FCtx.rsup Δ Δ' x = a → ∃b : α, Δ x = b := by
+  simp only [rsup_app]
   split <;> intro h <;> cases h; exact ⟨_, by assumption⟩
-theorem FCtx.rinf_var_right {Δ Δ' : FCtx ν α} (x : ν) (a : α)
-  : FCtx.rinf Δ Δ' x = a → Δ' x = a := by
-  simp only [rinf_app]
+theorem FCtx.rsup_var_right {Δ Δ' : FCtx ν α} (x : ν) (a : α)
+  : FCtx.rsup Δ Δ' x = a → Δ' x = a := by
+  simp only [rsup_app]
   split <;> intro h <;> cases h; assumption
 
-theorem FCtx.rinf_var_right_eq' {Δ Δ' : FCtx ν α} (x : ν) (a : α) (bb : WithBot α)
-  (h : FCtx.rinf Δ Δ' x = a) (h' : Δ' x = bb) : a = bb := by
-    rw [<-rinf_var_right x a h]; assumption
-theorem FCtx.rinf_var_right_eq {Δ Δ' : FCtx ν α} (x : ν) (a b : α)
-  (h : FCtx.rinf Δ Δ' x = a) (h' : Δ' x = b) : a = b := by
-    cases rinf_var_right_eq' x a b h h'; rfl
+theorem FCtx.rsup_var_right_eq' {Δ Δ' : FCtx ν α} (x : ν) (a : α) (bb : WithTop α)
+  (h : FCtx.rsup Δ Δ' x = a) (h' : Δ' x = bb) : a = bb := by
+    rw [<-rsup_var_right x a h]; assumption
+theorem FCtx.rsup_var_right_eq {Δ Δ' : FCtx ν α} (x : ν) (a b : α)
+  (h : FCtx.rsup Δ Δ' x = a) (h' : Δ' x = b) : a = b := by
+    cases rsup_var_right_eq' x a b h h'; rfl
 
-theorem FCtx.rinf_support_eq_right {Δ Δ' : FCtx ν α} (x : ν)
-  (h : x ∈ (rinf Δ Δ').support) : FCtx.rinf Δ Δ' x = Δ' x := (rinf_wk Δ Δ').eq_on x h
+theorem FCtx.rsup_support_eq_right {Δ Δ' : FCtx ν α} (x : ν)
+  (h : x ∈ (rsup Δ Δ').support) : FCtx.rsup Δ Δ' x = Δ' x := (rsup_wk Δ Δ').eq_on x h
 
-theorem FCtx.rinf_var_eq_right {Δ Δ' : FCtx ν α} (x : ν) (a : α)
-  (h : FCtx.rinf Δ Δ' x = a)
-  : FCtx.rinf Δ Δ' x = Δ' x := by
+theorem FCtx.rsup_var_eq_right {Δ Δ' : FCtx ν α} (x : ν) (a : α)
+  (h : FCtx.rsup Δ Δ' x = a)
+  : FCtx.rsup Δ Δ' x = Δ' x := by
     rw [h]
     apply Eq.symm
-    apply rinf_var_right
+    apply rsup_var_right
     exact h
-theorem FCtx.rinf_left_var_eq_right {Δ Δ' : FCtx ν α} (x : ν) (a : α)
+theorem FCtx.rsup_left_var_eq_right {Δ Δ' : FCtx ν α} (x : ν) (a : α)
   (h : Δ x = a)
-  : FCtx.rinf Δ Δ' x = Δ' x := by
-    rw [rinf_app]
+  : FCtx.rsup Δ Δ' x = Δ' x := by
+    rw [rsup_app]
     split
     . rw [h] at *; contradiction
-    . simp [*, Bot.bot] at *
+    . simp [*, Top.top] at *
     . simp [*]
 
-theorem FCtx.rinf_some_eq_right {Δ Δ' : FCtx ν α} (x : ν)
-: (∃a : α, FCtx.rinf Δ Δ' x = a) → FCtx.rinf Δ Δ' x = Δ' x := by
+theorem FCtx.rsup_some_eq_right {Δ Δ' : FCtx ν α} (x : ν)
+: (∃a : α, FCtx.rsup Δ Δ' x = a) → FCtx.rsup Δ Δ' x = Δ' x := by
   intro ⟨a, h⟩
   rw [h]
   apply Eq.symm
-  apply rinf_var_right
+  apply rsup_var_right
   exact h
-theorem FCtx.rinf_left_some_eq_right {Δ Δ' : FCtx ν α} (x : ν)
-  : (∃a: α, Δ x = a) → FCtx.rinf Δ Δ' x = Δ' x := by
+theorem FCtx.rsup_left_some_eq_right {Δ Δ' : FCtx ν α} (x : ν)
+  : (∃a: α, Δ x = a) → FCtx.rsup Δ Δ' x = Δ' x := by
   intro ⟨a, h⟩
-  apply rinf_left_var_eq_right _ _ h
-theorem FCtx.rinf_left_support_eq_right {Δ Δ' : FCtx ν α} (x : ν)
-  (h : x ∈ Δ.support) : FCtx.rinf Δ Δ' x = Δ' x := by
-  apply rinf_left_some_eq_right _ ((mem_support_exists _).mp h)
+  apply rsup_left_var_eq_right _ _ h
+theorem FCtx.rsup_left_support_eq_right {Δ Δ' : FCtx ν α} (x : ν)
+  (h : x ∈ Δ.support) : FCtx.rsup Δ Δ' x = Δ' x := by
+  apply rsup_left_some_eq_right _ ((mem_support_exists _).mp h)
   rfl
-theorem FCtx.rinf_right_not_support {Δ Δ' : FCtx ν α} (x : ν)
-  (h : x ∉ Δ.support) : FCtx.rinf Δ Δ' x = ⊥ := by
-  apply rinf_eq_none_left
-  apply eq_bot_of_not_mem_support
+theorem FCtx.rsup_right_not_support {Δ Δ' : FCtx ν α} (x : ν)
+  (h : x ∉ Δ.support) : FCtx.rsup Δ Δ' x = ⊤ := by
+  apply rsup_eq_none_left
+  apply eq_top_of_not_mem_support
   exact h
-theorem FCtx.rinf_eq_eq_right {Δ Δ' : FCtx ν α} (x : ν)
-  (h : Δ x = Δ' x) : FCtx.rinf Δ Δ' x = Δ' x := by
+theorem FCtx.rsup_eq_eq_right {Δ Δ' : FCtx ν α} (x : ν)
+  (h : Δ x = Δ' x) : FCtx.rsup Δ Δ' x = Δ' x := by
   if h': x ∈ Δ.support then
-    rw [rinf_left_support_eq_right _ h']
+    rw [rsup_left_support_eq_right _ h']
   else
-    rw [rinf_right_not_support _ h']
-    rw [eq_bot_of_not_mem_support _ h'] at h
+    rw [rsup_right_not_support _ h']
+    rw [eq_top_of_not_mem_support _ h'] at h
     rw [h]
-theorem FCtx.rinf_eq_eq_left {Δ Δ' : FCtx ν α} (x : ν)
-  (h : Δ x = Δ' x) : FCtx.rinf Δ Δ' x = Δ x := by
-    rw [rinf_eq_eq_right _ h]
+theorem FCtx.rsup_eq_eq_left {Δ Δ' : FCtx ν α} (x : ν)
+  (h : Δ x = Δ' x) : FCtx.rsup Δ Δ' x = Δ x := by
+    rw [rsup_eq_eq_right _ h]
     exact h.symm
 
-theorem FCtx.Wk.rinf_wk {Γ Δ Δ' : FCtx ν α} (w : FCtx.Wk Δ Γ) (w' : FCtx.Wk Δ' Γ)
-  : FCtx.Wk (FCtx.rinf Δ Δ') Γ := by
+theorem FCtx.Wk.rsup_wk {Γ Δ Δ' : FCtx ν α} (w : FCtx.Wk Δ Γ) (w' : FCtx.Wk Δ' Γ)
+  : FCtx.Wk (FCtx.rsup Δ Δ') Γ := by
   simp only [eq_on_iff] at *
   intro x hx
-  rw [rinf_eq_eq_left]
+  rw [rsup_eq_eq_left]
   . rw [<-w _ hx]
   . rw [<-w' _ hx]
     rw [<-w _ hx]
 
-theorem FCtx.linf_assoc (Δ₁ Δ₂ Δ₃ : FCtx ν α)
-  : FCtx.linf (FCtx.linf Δ₁ Δ₂) Δ₃ = FCtx.linf Δ₁ (FCtx.linf Δ₂ Δ₃) := by
+theorem FCtx.lsup_assoc (Δ₁ Δ₂ Δ₃ : FCtx ν α)
+  : FCtx.lsup (FCtx.lsup Δ₁ Δ₂) Δ₃ = FCtx.lsup Δ₁ (FCtx.lsup Δ₂ Δ₃) := by
   apply FCtx.ext
   intro x
   conv =>
     rhs
-    rw [linf_app]
+    rw [lsup_app]
   split
-  . apply linf_eq_none_left; apply linf_eq_none_left; assumption
-  . simp only [linf_eq_none_iff]
+  . apply lsup_eq_none_left; apply lsup_eq_none_left; assumption
+  . simp only [lsup_eq_none_iff]
     rw [or_assoc]
     apply Or.inr
-    apply linf_eq_none_or
+    apply lsup_eq_none_or
     assumption
   . rename_i h
-    rw [linf_right_some_eq_left _ (linf_var_right _ _ h)]
-    rw [linf_right_var_eq_left _ _ (linf_var_left _ _ h)]
+    rw [lsup_right_some_eq_left _ (lsup_var_right _ _ h)]
+    rw [lsup_right_var_eq_left _ _ (lsup_var_left _ _ h)]
     assumption
 
-theorem FCtx.rinf_assoc (Δ₁ Δ₂ Δ₃ : FCtx ν α)
-  : FCtx.rinf (FCtx.rinf Δ₁ Δ₂) Δ₃ = FCtx.rinf Δ₁ (FCtx.rinf Δ₂ Δ₃) := by
+theorem FCtx.rsup_assoc (Δ₁ Δ₂ Δ₃ : FCtx ν α)
+  : FCtx.rsup (FCtx.rsup Δ₁ Δ₂) Δ₃ = FCtx.rsup Δ₁ (FCtx.rsup Δ₂ Δ₃) := by
   apply FCtx.ext
   intro x
   conv =>
     rhs
-    rw [rinf_app]
+    rw [rsup_app]
   split
-  . apply rinf_eq_none_left; apply rinf_eq_none_left; assumption
-  . simp only [rinf_eq_none_iff]
+  . apply rsup_eq_none_left; apply rsup_eq_none_left; assumption
+  . simp only [rsup_eq_none_iff]
     rw [or_assoc]
     apply Or.inr
-    apply rinf_eq_none_or
+    apply rsup_eq_none_or
     assumption
   . rename_i h
-    have ⟨b, hb⟩ := rinf_var_left _ _ h;
-    rw [rinf_left_var_eq_right _ b]
-    exact rinf_var_right _ _ h
-    rw [rinf_left_var_eq_right _ _]
+    have ⟨b, hb⟩ := rsup_var_left _ _ h;
+    rw [rsup_left_var_eq_right _ b]
+    exact rsup_var_right _ _ h
+    rw [rsup_left_var_eq_right _ _]
     exact hb
     assumption
 
-theorem FCtx.linf_comm (Δ Δ' : FCtx ν α)
-  : FCtx.linf Δ Δ' = FCtx.rinf Δ' Δ := by
+theorem FCtx.lsup_comm (Δ Δ' : FCtx ν α)
+  : FCtx.lsup Δ Δ' = FCtx.rsup Δ' Δ := by
   apply FCtx.ext
   intro x;
-  simp only [linf_app, rinf_app]
+  simp only [lsup_app, rsup_app]
   split
   . split
     . rfl
@@ -628,154 +630,154 @@ theorem FCtx.linf_comm (Δ Δ' : FCtx ν α)
     . rename_i h _ _ _ _ _ _ h'
       rw [<-h, <-h']
 
-theorem FCtx.rinf_comm (Δ Δ' : FCtx ν α)
-  : FCtx.rinf Δ Δ' = FCtx.linf Δ' Δ := by
-  rw [linf_comm]
+theorem FCtx.rsup_comm (Δ Δ' : FCtx ν α)
+  : FCtx.rsup Δ Δ' = FCtx.lsup Δ' Δ := by
+  rw [lsup_comm]
 
-theorem FCtx.linf_idem (Δ : FCtx ν α)
-  : FCtx.linf Δ Δ = Δ := by
+theorem FCtx.lsup_idem (Δ : FCtx ν α)
+  : FCtx.lsup Δ Δ = Δ := by
   apply FCtx.ext
   intro x
-  simp only [linf_app]
-  split <;> simp [WithBot.bot, *]
+  simp only [lsup_app]
+  split <;> simp [WithTop.top, *]
 
-theorem FCtx.rinf_idem (Δ : FCtx ν α)
-  : FCtx.rinf Δ Δ = Δ := by
-  rw [<-(FCtx.Cmp.refl Δ).linf_eq_rinf, linf_idem]
+theorem FCtx.rsup_idem (Δ : FCtx ν α)
+  : FCtx.rsup Δ Δ = Δ := by
+  rw [<-(FCtx.Cmp.refl Δ).lsup_eq_rsup, lsup_idem]
 
---TODO: linf_nil, nil_linf, rinf_nil, nil_rinf
+--TODO: lsup_nil, nil_lsup, rsup_nil, nil_rsup
 
---TODO: inf eq iff wk
+--TODO: sup eq iff wk
 
-def FCtx.lsup (Δ Δ' : FCtx ν α)
+def FCtx.linf (Δ Δ' : FCtx ν α)
   : FCtx ν α where
   toFun x := match Δ x, Δ' x with
-    | ⊥, _ => Δ' x
-    | _, ⊥ => Δ x
+    | ⊤, _ => Δ' x
+    | _, ⊤ => Δ x
     | some a, some _ => some a
   support := Δ.support ∪ Δ'.support
   mem_support_toFun := by
     intro x
     simp only [Finset.mem_union, mem_support]
-    split <;> simp [Bot.bot, *]
+    split <;> simp [Top.top, *]
 
-theorem FCtx.lsup_app (Δ Δ' : FCtx ν α) (x : ν)
-  : (FCtx.lsup Δ Δ') x = match Δ x, Δ' x with
-    | ⊥, _ => Δ' x
-    | _, ⊥ => Δ x
+theorem FCtx.linf_app (Δ Δ' : FCtx ν α) (x : ν)
+  : (FCtx.linf Δ Δ') x = match Δ x, Δ' x with
+    | ⊤, _ => Δ' x
+    | _, ⊤ => Δ x
     | some a, some _ => some a := by rfl
 
-theorem FCtx.lsup_support {Δ Δ' : FCtx ν α}
-  : (FCtx.lsup Δ Δ').support = Δ.support ∪ Δ'.support := rfl
+theorem FCtx.linf_support {Δ Δ' : FCtx ν α}
+  : (FCtx.linf Δ Δ').support = Δ.support ∪ Δ'.support := rfl
 
-def FCtx.rsup (Δ Δ' : FCtx ν α)
+def FCtx.rinf (Δ Δ' : FCtx ν α)
   : FCtx ν α where
   toFun x := match Δ x, Δ' x with
-    | ⊥, _ => Δ' x
-    | _, ⊥ => Δ x
+    | ⊤, _ => Δ' x
+    | _, ⊤ => Δ x
     | some _, some a => some a
   support := Δ.support ∪ Δ'.support
   mem_support_toFun := by
     intro x
     simp only [Finset.mem_union, mem_support]
-    split <;> simp [Bot.bot, *]
+    split <;> simp [Top.top, *]
 
-theorem FCtx.rsup_app (Δ Δ' : FCtx ν α) (x : ν)
-  : (FCtx.rsup Δ Δ') x = match Δ x, Δ' x with
-    | ⊥, _ => Δ' x
-    | _, ⊥ => Δ x
+theorem FCtx.rinf_app (Δ Δ' : FCtx ν α) (x : ν)
+  : (FCtx.rinf Δ Δ') x = match Δ x, Δ' x with
+    | ⊤, _ => Δ' x
+    | _, ⊤ => Δ x
     | some _, some a => some a := by rfl
 
-theorem FCtx.rsup_support {Δ Δ' : FCtx ν α}
-  : (FCtx.rsup Δ Δ').support = Δ.support ∪ Δ'.support := rfl
+theorem FCtx.rinf_support {Δ Δ' : FCtx ν α}
+  : (FCtx.rinf Δ Δ').support = Δ.support ∪ Δ'.support := rfl
 
-theorem FCtx.lsup_wk (Δ Δ' : FCtx ν α) : FCtx.Wk (FCtx.lsup Δ Δ') Δ := by
+theorem FCtx.linf_wk (Δ Δ' : FCtx ν α) : FCtx.Wk (FCtx.linf Δ Δ') Δ := by
   intro x
-  simp [lsup_app]
-  split <;> simp [Bot.bot, *]
+  simp [linf_app]
+  split <;> simp [Top.top, *]
 
-theorem FCtx.rsup_wk (Δ Δ' : FCtx ν α) : FCtx.Wk (FCtx.rsup Δ Δ') Δ' := by
+theorem FCtx.rinf_wk (Δ Δ' : FCtx ν α) : FCtx.Wk (FCtx.rinf Δ Δ') Δ' := by
   intro x
-  simp [rsup_app]
-  split <;> simp [Bot.bot, *]
+  simp [rinf_app]
+  split <;> simp [Top.top, *]
 
-theorem FCtx.Cmp.lsup_eq_rsup {Δ Δ' : FCtx ν α} (c : FCtx.Cmp Δ Δ')
-  : FCtx.lsup Δ Δ' = FCtx.rsup Δ Δ' := by
+theorem FCtx.Cmp.linf_eq_rinf {Δ Δ' : FCtx ν α} (c : FCtx.Cmp Δ Δ')
+  : FCtx.linf Δ Δ' = FCtx.rinf Δ Δ' := by
   apply FCtx.ext
   intro x
-  simp only [DFunLike.coe, lsup, rsup]
+  simp only [DFunLike.coe, linf, rinf]
   split
   . rfl
   . rfl
   . apply var_eq' c <;> assumption
 
-theorem FCtx.Wk.lsup_eq_rsup {Γ Δ Δ' : FCtx ν α} (w : FCtx.Wk Γ Δ) (w' : FCtx.Wk Γ Δ')
-  : FCtx.lsup Δ Δ' = FCtx.rsup Δ Δ' := (w.cmp₂ w').lsup_eq_rsup
+theorem FCtx.Wk.linf_eq_rinf {Γ Δ Δ' : FCtx ν α} (w : FCtx.Wk Γ Δ) (w' : FCtx.Wk Γ Δ')
+  : FCtx.linf Δ Δ' = FCtx.rinf Δ Δ' := (w.cmp₂ w').linf_eq_rinf
 
-theorem FCtx.Cmp.lsup_wk_left {Δ Δ' : FCtx ν α} (_ : FCtx.Cmp Δ Δ')
-  : FCtx.Wk (FCtx.lsup Δ Δ') Δ := lsup_wk Δ Δ'
-theorem FCtx.Cmp.lsup_wk_right {Δ Δ' : FCtx ν α} (c : FCtx.Cmp Δ Δ')
-  : FCtx.Wk (FCtx.lsup Δ Δ') Δ' := c.lsup_eq_rsup ▸ rsup_wk Δ Δ'
+theorem FCtx.Cmp.linf_wk_left {Δ Δ' : FCtx ν α} (_ : FCtx.Cmp Δ Δ')
+  : FCtx.Wk (FCtx.linf Δ Δ') Δ := linf_wk Δ Δ'
+theorem FCtx.Cmp.linf_wk_right {Δ Δ' : FCtx ν α} (c : FCtx.Cmp Δ Δ')
+  : FCtx.Wk (FCtx.linf Δ Δ') Δ' := c.linf_eq_rinf ▸ rinf_wk Δ Δ'
 
-theorem FCtx.Wk.lsup_wk_left {Γ Δ Δ' : FCtx ν α} (_ : FCtx.Wk Γ Δ) (_ : FCtx.Wk Γ Δ')
-  : FCtx.Wk (FCtx.lsup Δ Δ') Δ := lsup_wk Δ Δ'
-theorem FCtx.Wk.lsup_wk_right {Γ Δ Δ' : FCtx ν α} (w : FCtx.Wk Γ Δ) (w' : FCtx.Wk Γ Δ')
-  : FCtx.Wk (FCtx.lsup Δ Δ') Δ' := lsup_eq_rsup w w' ▸ rsup_wk Δ Δ'
+theorem FCtx.Wk.linf_wk_left {Γ Δ Δ' : FCtx ν α} (_ : FCtx.Wk Γ Δ) (_ : FCtx.Wk Γ Δ')
+  : FCtx.Wk (FCtx.linf Δ Δ') Δ := linf_wk Δ Δ'
+theorem FCtx.Wk.linf_wk_right {Γ Δ Δ' : FCtx ν α} (w : FCtx.Wk Γ Δ) (w' : FCtx.Wk Γ Δ')
+  : FCtx.Wk (FCtx.linf Δ Δ') Δ' := linf_eq_rinf w w' ▸ rinf_wk Δ Δ'
 
-theorem FCtx.Cmp.rsup_wk_left {Δ Δ' : FCtx ν α} (c : FCtx.Cmp Δ Δ')
-  : FCtx.Wk (FCtx.rsup Δ Δ') Δ := c.lsup_eq_rsup ▸ lsup_wk Δ Δ'
-theorem FCtx.Cmp.rsup_wk_right {Δ Δ' : FCtx ν α} (_ : FCtx.Cmp Δ Δ')
-  : FCtx.Wk (FCtx.rsup Δ Δ') Δ' := rsup_wk Δ Δ'
+theorem FCtx.Cmp.rinf_wk_left {Δ Δ' : FCtx ν α} (c : FCtx.Cmp Δ Δ')
+  : FCtx.Wk (FCtx.rinf Δ Δ') Δ := c.linf_eq_rinf ▸ linf_wk Δ Δ'
+theorem FCtx.Cmp.rinf_wk_right {Δ Δ' : FCtx ν α} (_ : FCtx.Cmp Δ Δ')
+  : FCtx.Wk (FCtx.rinf Δ Δ') Δ' := rinf_wk Δ Δ'
 
-theorem FCtx.Wk.rsup_wk_left {Γ Δ Δ' : FCtx ν α} (w : FCtx.Wk Γ Δ) (w' : FCtx.Wk Γ Δ')
-  : FCtx.Wk (FCtx.rsup Δ Δ') Δ := lsup_eq_rsup w w' ▸ lsup_wk Δ Δ'
-theorem FCtx.Wk.rsup_wk_right {Γ Δ Δ' : FCtx ν α} (_ : FCtx.Wk Γ Δ) (_ : FCtx.Wk Γ Δ')
-  : FCtx.Wk (FCtx.rsup Δ Δ') Δ' := rsup_wk Δ Δ'
+theorem FCtx.Wk.rinf_wk_left {Γ Δ Δ' : FCtx ν α} (w : FCtx.Wk Γ Δ) (w' : FCtx.Wk Γ Δ')
+  : FCtx.Wk (FCtx.rinf Δ Δ') Δ := linf_eq_rinf w w' ▸ linf_wk Δ Δ'
+theorem FCtx.Wk.rinf_wk_right {Γ Δ Δ' : FCtx ν α} (_ : FCtx.Wk Γ Δ) (_ : FCtx.Wk Γ Δ')
+  : FCtx.Wk (FCtx.rinf Δ Δ') Δ' := rinf_wk Δ Δ'
 
 --TODO: wk lemmas, assoc, idem, nil, etc.
 
 theorem FCtx.Cmp.iff_exists_wk {Δ Δ' : FCtx ν α}
   : FCtx.Cmp Δ Δ' ↔ ∃Γ : FCtx ν α, Γ.Wk Δ ∧ Γ.Wk Δ'
-  := ⟨λc => ⟨_, c.lsup_wk_left, c.lsup_wk_right⟩, λ⟨_, w, w'⟩ => w.cmp₂ w'⟩
+  := ⟨λc => ⟨_, c.linf_wk_left, c.linf_wk_right⟩, λ⟨_, w, w'⟩ => w.cmp₂ w'⟩
 
-def FCtx.inf (Δ Δ' : FCtx ν α) : FCtx ν α where
-  toFun x := if Δ x = Δ' x then Δ x else ⊥
+def FCtx.sup (Δ Δ' : FCtx ν α) : FCtx ν α where
+  toFun x := if Δ x = Δ' x then Δ x else ⊤
   support := Δ.support.filter (λx => Δ x = Δ' x)
   mem_support_toFun := by
     intro x
     simp [mem_support_toFun]
     exact ⟨λh => ⟨h.2, h.1⟩, λh => ⟨h.2, h.1⟩⟩
 
-theorem FCtx.inf_support_left {Δ Δ' : FCtx ν α}
-  : (FCtx.inf Δ Δ').support = Δ.support.filter (λx => Δ x = Δ' x) := rfl
+theorem FCtx.sup_support_left {Δ Δ' : FCtx ν α}
+  : (FCtx.sup Δ Δ').support = Δ.support.filter (λx => Δ x = Δ' x) := rfl
 
-theorem FCtx.inf_comm (Δ Δ' : FCtx ν α)
-  : FCtx.inf Δ Δ' = FCtx.inf Δ' Δ := by
+theorem FCtx.sup_comm (Δ Δ' : FCtx ν α)
+  : FCtx.sup Δ Δ' = FCtx.sup Δ' Δ := by
   apply FCtx.ext
   intro x
-  simp only [DFunLike.coe, inf]
+  simp only [DFunLike.coe, sup]
   split
   . simp [*]
   . split
     . simp [*] at *
     . rfl
 
---TODO: inf_assoc
---TODO: inf_idem
---TODO: inf_nil
+--TODO: sup_assoc
+--TODO: sup_idem
+--TODO: sup_nil
 
-theorem FCtx.inf_support_right {Δ Δ' : FCtx ν α}
-  : (FCtx.inf Δ Δ').support = Δ'.support.filter (λx => Δ x = Δ' x) := by
-  rw [inf_comm, inf_support_left]
+theorem FCtx.sup_support_right {Δ Δ' : FCtx ν α}
+  : (FCtx.sup Δ Δ').support = Δ'.support.filter (λx => Δ x = Δ' x) := by
+  rw [sup_comm, sup_support_left]
   congr
   funext x
   apply propext; constructor <;> intro h <;> rw [h]
 
-theorem FCtx.Cmp.inf_eq_linf {Δ Δ' : FCtx ν α} (c : FCtx.Cmp Δ Δ')
-  : FCtx.inf Δ Δ' = FCtx.linf Δ Δ' := by
+theorem FCtx.Cmp.sup_eq_lsup {Δ Δ' : FCtx ν α} (c : FCtx.Cmp Δ Δ')
+  : FCtx.sup Δ Δ' = FCtx.lsup Δ Δ' := by
   apply FCtx.ext
   intro x
-  simp only [DFunLike.coe, inf, linf]
+  simp only [DFunLike.coe, sup, lsup]
   split
   . rename_i h
     simp [h]
@@ -788,8 +790,8 @@ theorem FCtx.Cmp.inf_eq_linf {Δ Δ' : FCtx ν α} (c : FCtx.Cmp Δ Δ')
       | Or.inr (Or.inl h) => cases hΔ.symm.trans h
       | Or.inr (Or.inr h) => cases hΔ'.symm.trans h
 
-theorem FCtx.Cmp.inf_eq_rinf {Δ Δ' : FCtx ν α} (c : FCtx.Cmp Δ Δ')
-  : FCtx.inf Δ Δ' = FCtx.rinf Δ Δ' := by rw [c.inf_eq_linf, c.linf_eq_rinf]
+theorem FCtx.Cmp.sup_eq_rsup {Δ Δ' : FCtx ν α} (c : FCtx.Cmp Δ Δ')
+  : FCtx.sup Δ Δ' = FCtx.rsup Δ Δ' := by rw [c.sup_eq_lsup, c.lsup_eq_rsup]
 
 --TODO: instantiate semilattice structure
 
@@ -806,24 +808,24 @@ theorem FCtx.Cmp.eq_of_eq_support {Δ Δ' : FCtx ν α} (c : FCtx.Cmp Δ Δ')
   | Or.inr (Or.inl hx) =>
     rw [hx]
     apply Eq.symm
-    apply eq_bot_of_not_mem_support
+    apply eq_top_of_not_mem_support
     intro hx'
     rw [<-h] at hx'
-    exact not_mem_support_of_eq_bot _ hx hx'
+    exact not_mem_support_of_eq_top _ hx hx'
   | Or.inr (Or.inr hx) =>
     rw [hx]
-    apply eq_bot_of_not_mem_support
+    apply eq_top_of_not_mem_support
     intro hx'
     rw [h] at hx'
-    exact not_mem_support_of_eq_bot _ hx hx'
+    exact not_mem_support_of_eq_top _ hx hx'
 
 def FCtx.restrict (Γ : FCtx ν α) (vars : Finset ν) : FCtx ν α where
-  toFun x := if x ∈ vars then Γ x else ⊥
+  toFun x := if x ∈ vars then Γ x else ⊤
   support := Γ.support ∩ vars
   mem_support_toFun := by simp [mem_support, And.comm]
 
 theorem FCtx.restrict_app (Γ : FCtx ν α) (vars : Finset ν) (x : ν)
-  : (FCtx.restrict Γ vars) x = if x ∈ vars then Γ x else ⊥
+  : (FCtx.restrict Γ vars) x = if x ∈ vars then Γ x else ⊤
   := rfl
 
 theorem FCtx.restrict_support (Γ : FCtx ν α) : Γ.restrict Γ.support = Γ
@@ -913,7 +915,7 @@ theorem FCtx.Wk.restrict {Γ Δ : FCtx ν α} (w : Γ.Wk Δ) (v : Finset ν)
 --TODO: in a coherent setting, any two contexts typing a term have equal restrictions
 
 def FCtx.erase (Γ : FCtx ν α) (x : ν) : FCtx ν α where
-  toFun y := if y = x then ⊥ else Γ y
+  toFun y := if y = x then ⊤ else Γ y
   support := Γ.support.erase x
   mem_support_toFun := by
     intro y
@@ -921,7 +923,7 @@ def FCtx.erase (Γ : FCtx ν α) (x : ν) : FCtx ν α where
     split <;> simp [*]
 
 theorem FCtx.erase_app (Γ : FCtx ν α) (x y : ν)
-  : (FCtx.erase Γ x) y = if y = x then ⊥ else Γ y := rfl
+  : (FCtx.erase Γ x) y = if y = x then ⊤ else Γ y := rfl
 
 theorem FCtx.erase_eq (Γ : FCtx ν α) (x : ν) (hx : x ∉ Γ.support)
   : FCtx.erase Γ x = Γ := by
@@ -930,7 +932,7 @@ theorem FCtx.erase_eq (Γ : FCtx ν α) (x : ν) (hx : x ∉ Γ.support)
   simp only [erase_app, ite_eq_right_iff]
   intro hy
   cases hy
-  rw [eq_bot_of_not_mem_support _ hx]
+  rw [eq_top_of_not_mem_support _ hx]
 
 theorem FCtx.Wk.of_erase (Γ : FCtx ν α) (x : ν) : Γ.Wk (Γ.erase x) := by
   intro y
@@ -938,7 +940,7 @@ theorem FCtx.Wk.of_erase (Γ : FCtx ν α) (x : ν) : Γ.Wk (Γ.erase x) := by
   split <;> simp [Bot.bot, *]
 
 def FCtx.sdiff (Γ : FCtx ν α) (N : Finset ν) : FCtx ν α where
-  toFun x := if x ∈ N then ⊥ else Γ x
+  toFun x := if x ∈ N then ⊤ else Γ x
   support := Γ.support \ N
   mem_support_toFun := by
     intro x
@@ -946,7 +948,7 @@ def FCtx.sdiff (Γ : FCtx ν α) (N : Finset ν) : FCtx ν α where
     split <;> simp [*]
 
 theorem FCtx.sdiff_app (Γ : FCtx ν α) (N : Finset ν) (x : ν)
-  : (FCtx.sdiff Γ N) x = if x ∈ N then ⊥ else Γ x := rfl
+  : (FCtx.sdiff Γ N) x = if x ∈ N then ⊤ else Γ x := rfl
 
 theorem FCtx.sdiff_eq_restrict (Γ : FCtx ν α) (N : Finset ν)
   : FCtx.sdiff Γ N = Γ.restrict (Γ.support \ N) := by
@@ -968,7 +970,7 @@ theorem FCtx.sdiff_eq (Γ : FCtx ν α) (N : Finset ν) (hΓ : Disjoint Γ.suppo
   split
   . rename_i hx
     apply Eq.symm
-    apply eq_bot_of_not_mem_support
+    apply eq_top_of_not_mem_support
     intro hx'
     apply Finset.disjoint_iff_ne.mp <;> first | assumption | rfl
   . rfl
@@ -988,7 +990,7 @@ theorem FCtx.Wk.sdiff {Γ Δ : FCtx ν α} (w : Γ.Wk Δ) (N : Finset ν)
   : (Γ.sdiff N).Wk (Δ.sdiff N) := by
   intro x
   simp only [sdiff_app]
-  split <;> simp only [Bot.bot, or_self]
+  split <;> simp only [Top.top, or_self]
   exact w x
 
 --TODO: sdiff_eq_erase for singleton, etc...
